Refactor SemanticEval to receive only one SemanticStore (#213)
*Description of changes:*

This pull request updates the expression evaluator (`SemanticEval` in
Strata) which previously needed to take two states: one for old
expressions, one for normal (‘new’) expressions, but after this pull
request it takes only one state.
It introduces a couple of `sorry`s, but these will be eventually fixed.

By submitting this pull request, I confirm that you can use, modify,
copy, and redistribute this contribution, under the terms of your
choice.

Strata/DL/Imperative/CmdSemantics.lean
@@ -24,8 +24,8 @@ lookups. The evaluation functions take two states: an old state and a
 current state. This allows for two-state expressions and predicates.
 -/
 abbrev SemanticStore := P.Ident → Option P.Expr
-abbrev SemanticEval := SemanticStore P → SemanticStore P → P.Expr → Option P.Expr
-abbrev SemanticEvalBool := SemanticStore P → SemanticStore P → P.Expr → Option Bool
+abbrev SemanticEval := SemanticStore P → P.Expr → Option P.Expr
+abbrev SemanticEvalBool := SemanticStore P → P.Expr → Option Bool
 
 
 /--
@@ -33,8 +33,7 @@ Evaluation relation of an Imperative command `Cmd`.
 -/
 -- (FIXME) Change to a type class?
 abbrev EvalCmdParam (P : PureExpr) (Cmd : Type) :=
-  SemanticEval P → SemanticStore P → SemanticStore P → Cmd →
-  SemanticStore P → Prop
+  SemanticEval P → SemanticStore P → Cmd → SemanticStore P → Prop
 
 /-- ### Well-Formedness of `SemanticStore`s -/
 
@@ -219,22 +218,22 @@ theorem invStoresExceptComm :
   -/
 def WellFormedSemanticEvalBool {P : PureExpr} [HasBool P] [HasNot P]
     (δ : SemanticEval P) : Prop :=
-    ∀ σ₀ σ e,
-      (δ σ₀ σ e = some Imperative.HasBool.tt ↔ δ σ₀ σ (Imperative.HasNot.not e) = (some HasBool.ff)) ∧
-      (δ σ₀ σ e = some Imperative.HasBool.ff ↔ δ σ₀ σ (Imperative.HasNot.not e) = (some HasBool.tt))
+    ∀ σ e,
+      (δ σ e = some Imperative.HasBool.tt ↔ δ σ (Imperative.HasNot.not e) = (some HasBool.ff)) ∧
+      (δ σ e = some Imperative.HasBool.ff ↔ δ σ (Imperative.HasNot.not e) = (some HasBool.tt))
 
 def WellFormedSemanticEvalVal {P : PureExpr} [HasVal P]
     (δ : SemanticEval P) : Prop :=
   -- evaluator only evaluates to values
-    (∀ v v' σ₀ σ, δ σ₀ σ v = some v' → HasVal.value v') ∧
+    (∀ v v' σ, δ σ v = some v' → HasVal.value v') ∧
   -- evaluator is identity on values
-    (∀ v' σ₀ σ, HasVal.value v' → δ σ₀ σ v' = some v')
+    (∀ v' σ, HasVal.value v' → δ σ v' = some v')
 
 def WellFormedSemanticEvalVar {P : PureExpr} [HasFvar P] (δ : SemanticEval P)
-    : Prop := (∀ e v σ₀ σ, HasFvar.getFvar e = some v → δ σ₀ σ e = σ v)
+    : Prop := (∀ e v σ, HasFvar.getFvar e = some v → δ σ e = σ v)
 
 def WellFormedSemanticEvalExprCongr {P : PureExpr} [HasVarsPure P P.Expr] (δ : SemanticEval P)
-    : Prop := ∀ e σ₀ σ σ', (∀ x ∈ HasVarsPure.getVars e, σ x = σ' x) → δ σ₀ σ e = δ σ₀ σ' e
+    : Prop := ∀ e σ σ', (∀ x ∈ HasVarsPure.getVars e, σ x = σ' x) → δ σ e = δ σ' e
 /--
 An inductive rule for state update.
 -/
@@ -262,38 +261,38 @@ An inductively-defined operational semantics that depends on
 environment lookup and evaluation functions for expressions.
 -/
 inductive EvalCmd [HasFvar P] [HasBool P] [HasNot P] :
-  SemanticEval P → SemanticStore P → SemanticStore P → Cmd P → SemanticStore P → Prop where
+  SemanticEval P → SemanticStore P → Cmd P → SemanticStore P → Prop where
   | eval_init :
-    δ σ₀ σ e = .some v →
+    δ σ e = .some v →
     InitState P σ x v σ' →
     WellFormedSemanticEvalVar δ →
     ---
-    EvalCmd δ σ₀ σ (.init x _ e _) σ'
+    EvalCmd δ σ (.init x _ e _) σ'
 
   | eval_set :
-    δ σ₀ σ e = .some v →
+    δ σ e = .some v →
     UpdateState P σ x v σ' →
     WellFormedSemanticEvalVar δ →
     ----
-    EvalCmd δ σ₀ σ (.set x e _) σ'
+    EvalCmd δ σ (.set x e _) σ'
 
   | eval_havoc :
     UpdateState P σ x v σ' →
     WellFormedSemanticEvalVar δ →
     ----
-    EvalCmd δ σ₀ σ (.havoc x _) σ'
+    EvalCmd δ σ (.havoc x _) σ'
 
   | eval_assert :
-    δ σ₀ σ e = .some HasBool.tt →
+    δ σ e = .some HasBool.tt →
     WellFormedSemanticEvalBool δ →
     ----
-    EvalCmd δ σ₀ σ (.assert _ e _) σ
+    EvalCmd δ σ (.assert _ e _) σ
 
   | eval_assume :
-    δ σ₀ σ e = .some HasBool.tt →
+    δ σ e = .some HasBool.tt →
     WellFormedSemanticEvalBool δ →
     ----
-    EvalCmd δ σ₀ σ (.assume _ e _) σ
+    EvalCmd δ σ (.assume _ e _) σ
 
 end section
 
