Strata/DL/Imperative/NondetStmtSemantics.lean
@@ -18,32 +18,31 @@ statements that depends on environment lookup and evaluation functions
 for expressions.  -/
 inductive EvalNondetStmt (P : PureExpr) (Cmd : Type) (EvalCmd : EvalCmdParam P Cmd)
   [HasVarsImp P (List (Stmt P Cmd))] [HasVarsImp P Cmd] [HasFvar P] [HasBool P] [HasNot P] :
-  SemanticEval P → SemanticStore P → SemanticStore P →
-    NondetStmt P Cmd → SemanticStore P → Prop where
+  SemanticEval P → SemanticStore P → NondetStmt P Cmd → SemanticStore P → Prop where
   | cmd_sem :
-    EvalCmd δ σ₀ σ c σ' →
+    EvalCmd δ σ c σ' →
     -- We only require definedness on the statement level so that the requirement is fine-grained
     isDefinedOver (HasVarsImp.modifiedVars) σ c →
     ----
-    EvalNondetStmt P Cmd EvalCmd δ σ₀ σ (NondetStmt.cmd c) σ'
+    EvalNondetStmt P Cmd EvalCmd δ σ (NondetStmt.cmd c) σ'
 
   | seq_sem :
-    EvalNondetStmt P Cmd EvalCmd δ σ₀ σ s1 σ' →
-    EvalNondetStmt P Cmd EvalCmd δ σ₀ σ' s2 σ'' →
+    EvalNondetStmt P Cmd EvalCmd δ σ s1 σ' →
+    EvalNondetStmt P Cmd EvalCmd δ σ' s2 σ'' →
     ----
-    EvalNondetStmt P Cmd EvalCmd δ σ₀ σ (.seq s1 s2) σ''
+    EvalNondetStmt P Cmd EvalCmd δ σ (.seq s1 s2) σ''
 
   | choice_left_sem :
     WellFormedSemanticEvalBool δ →
-    EvalNondetStmt P Cmd EvalCmd δ σ₀ σ s1 σ' →
+    EvalNondetStmt P Cmd EvalCmd δ σ s1 σ' →
     ----
-    EvalNondetStmt P Cmd EvalCmd δ σ₀ σ (.choice s1 s2) σ'
+    EvalNondetStmt P Cmd EvalCmd δ σ (.choice s1 s2) σ'
 
   | choice_right_sem :
     WellFormedSemanticEvalBool δ →
-    EvalNondetStmt P Cmd EvalCmd δ σ₀ σ s2 σ' →
+    EvalNondetStmt P Cmd EvalCmd δ σ s2 σ' →
     ----
-    EvalNondetStmt P Cmd EvalCmd δ σ₀ σ (.choice s1 s2) σ'
+    EvalNondetStmt P Cmd EvalCmd δ σ (.choice s1 s2) σ'
 
   /-
   | loop_sem :
